src/NLustreToStc/NL2StcNormalArgs.v
@@ -13,11 +13,12 @@ Module Type NL2STCNORMALARGS
        (Import Ids   : IDS)
        (Import Op    : OPERATORS)
        (Import OpAux : OPERATORS_AUX   Op)
+       (Import Strs  : STREAMS         Op OpAux)
        (Import Str   : STREAM          Op OpAux)
-       (Import CE    : COREEXPR    Ids Op OpAux Str)
-       (Import NL    : NLUSTRE     Ids Op OpAux Str CE)
-       (Import Stc   : STC         Ids Op OpAux Str CE)
-       (Import Trans : TRANSLATION Ids Op       CE.Syn NL.Syn Stc.Syn NL.Mem).
+       (Import CE    : COREEXPR    Ids Op OpAux      Str)
+       (Import NL    : NLUSTRE     Ids Op OpAux Strs Str CE)
+       (Import Stc   : STC         Ids Op OpAux      Str CE)
+       (Import Trans : TRANSLATION Ids Op                CE.Syn NL.Syn Stc.Syn NL.Mem).
 
   Lemma translate_eqn_normal_args:
     forall G eq,
@@ -57,11 +58,12 @@ Module NL2StcNormalArgsFun
        (Ids   : IDS)
        (Op    : OPERATORS)
        (OpAux : OPERATORS_AUX   Op)
+       (Strs  : STREAMS         Op OpAux)
        (Str   : STREAM          Op OpAux)
-       (CE    : COREEXPR    Ids Op OpAux Str)
-       (NL    : NLUSTRE     Ids Op OpAux Str CE)
-       (Stc   : STC         Ids Op OpAux Str CE)
-       (Trans : TRANSLATION Ids Op       CE.Syn NL.Syn Stc.Syn NL.Mem)
-<: NL2STCNORMALARGS Ids Op OpAux Str CE NL Stc Trans.
-  Include NL2STCNORMALARGS Ids Op OpAux Str CE NL Stc Trans.
+       (CE    : COREEXPR    Ids Op OpAux      Str)
+       (NL    : NLUSTRE     Ids Op OpAux Strs Str CE)
+       (Stc   : STC         Ids Op OpAux      Str CE)
+       (Trans : TRANSLATION Ids Op                CE.Syn NL.Syn Stc.Syn NL.Mem)
+<: NL2STCNORMALARGS Ids Op OpAux Strs Str CE NL Stc Trans.
+  Include NL2STCNORMALARGS Ids Op OpAux Strs Str CE NL Stc Trans.
 End NL2StcNormalArgsFun.
